riscV/CompilerAux.v
@@ -36,179 +36,19 @@ Qed.
   (** TargetPrinter *)
 Definition targetprinter p: res Asm.program :=
   OK p
-  (* @@ time "SSAsm" SSAsmproof.transf_program *)
-  (* @@@ time "Translation from SSAsm to RealAsm" RealAsmgen.transf_program instr_size *)
   @@ time "Elimination of pseudo instruction" PseudoInstructions.transf_program
   @@ time "Adjustment of float point arguments passing by fix-up code" AsmFixupcode.transf_program
   @@@ time "Expand builtin inline assembly" AsmBuiltinInline.transf_program
-  (* @@@ time "Pad Instructions with struct return" AsmStructRet.transf_program *)
-  (* @@ time "Generation of the float literal" AsmFloatLiteral.transf_program *)
-  (* @@ time "Generation of int64 literal" AsmLongInt.transf_program (* enable only in 64bit mode?  *) *)
   @@ time "Generation of the literal" AsmLiteral.transf_program
   @@ time "Elimination of other pseudo instructions" AsmPseudoInstr.transf_program
   @@@ time "Make local jumps use offsets instead of labels" Asmlabelgen.transf_program instr_size
   @@ time "Generation of the jump table" Jumptablegen.transf_program instr_size.
 
- (* verified part from SACompcert *)
-  (* Definition transf_c_program_real1 p: res Asm.program := *)
-  (* transf_c_program p *)
-  (* @@ time "SSAsm" SSAsmproof.transf_program *)
-  (* @@@ time "Translation from SSAsm to RealAsm" RealAsmgen.transf_program instr_size. *)
-
-
-
- (* without target printet, used to prove top theorem *)
- (* Definition transf_c_program_assembler1 (p: Csyntax.program) := *)
- (*  transf_c_program_real1 p *)
- (*  @@@ time "Generation of symbol table" Symbtablegen.transf_program instr_size *)
- (*  @@@ time "Generation of relocation table" Reloctablesgen.transf_program instr_size *)
- (*  @@@ time "Encoding of instructions and data" RelocBingen.transf_program *)
- (*  (* @@@ time "Merge Sections" MergeSection.transf_program *) *)
- (*  @@@ time "Generation of the reloctable Elf" RelocElfgen.gen_reloc_elf *)
- (*  @@@ time "Encoding of the reloctable Elf" EncodeRelocElf.encode_elf_file. *)
-
 Definition match_prog_targetprinter p tp :=
   targetprinter p = OK tp.
 
-
-Lemma Pseudo_fn_stack_requirements_match: forall p,
-    fn_stack_requirements p = fn_stack_requirements (PseudoInstructions.transf_program p).
-Proof.
-  intros. unfold fn_stack_requirements.  
-  eapply Axioms.extensionality. intros.
-  destr.
-  - eapply Globalenvs.Genv.find_funct_ptr_transf in Heqo.
-    erewrite Heqo.
-    2: {
-      instantiate (1:= PseudoInstructions.transf_fundef).
-      unfold PseudoInstructions.transf_program.
-      eapply match_transform_program. }
-    unfold PseudoInstructions.transf_fundef,PseudoInstructions.transf_function,transf_fundef.
-    destruct f. auto. auto.
-  - eapply match_program_no_more_functions in Heqo.
-    erewrite Heqo. auto.
-    eapply match_transform_program.
-Qed.
-
-Lemma Fixup_fn_stack_requirements_match: forall p,
-    fn_stack_requirements p = fn_stack_requirements (AsmFixupcode.transf_program p).
-Proof.
-  intros. unfold fn_stack_requirements.  
-  eapply Axioms.extensionality. intros.
-  destr.
-  - eapply Globalenvs.Genv.find_funct_ptr_transf in Heqo.
-    erewrite Heqo.
-    2: {
-      instantiate (1:= AsmFixupcode.transf_fundef).
-      unfold AsmFixupcode.transf_program.
-      eapply match_transform_program. }
-    unfold AsmFixupcode.transf_fundef,AsmFixupcode.transf_function,transf_fundef.
-    destruct f. auto. auto.
-  - eapply match_program_no_more_functions in Heqo.
-    erewrite Heqo. auto.
-    eapply match_transform_program.
-Qed.
-
-
-Lemma BuiltInline_fn_stack_requirements_match: forall p tp,
-    AsmBuiltinInline.transf_program p = OK tp ->
-    fn_stack_requirements p = fn_stack_requirements tp.
-Proof.
-  intros. unfold fn_stack_requirements.  
-  eapply Axioms.extensionality. intros.
-  destr.
-  - eapply Globalenvs.Genv.find_funct_ptr_transf_partial in Heqo.
-    destruct Heqo as (tf & A & B).
-    erewrite A.
-    2:{
-      instantiate (1:= AsmBuiltinInline.transf_fundef).
-      eapply match_transform_partial_program.
-      unfold AsmBuiltinInline.transf_program in H. auto.
-    }
-    unfold AsmBuiltinInline.transf_fundef,transf_partial_fundef,AsmBuiltinInline.transf_function,transf_fundef in B.
-    destruct f. monadInv B. monadInv EQ. auto. inv B. auto.
-  - eapply match_program_no_more_functions in Heqo.
-    erewrite Heqo. auto.
-    eapply match_transform_partial_program.
-    unfold AsmBuiltinInline.transf_program in H. eauto.
-Qed.    
-    
-Lemma AsmPseudo_fn_stack_requirements_match: forall p,
-    fn_stack_requirements p = fn_stack_requirements (AsmPseudoInstr.transf_program p).
-Proof.
-  intros. unfold fn_stack_requirements.  
-  eapply Axioms.extensionality. intros.
-  destr.
-  - eapply Globalenvs.Genv.find_funct_ptr_transf in Heqo.
-    erewrite Heqo.
-    2: {
-      instantiate (1:= AsmPseudoInstr.transf_fundef).
-      unfold AsmPseudoInstr.transf_program.
-      eapply match_transform_program. }
-    unfold AsmPseudoInstr.transf_fundef,AsmPseudoInstr.transf_function,transf_fundef.
-    destruct f. auto. auto.
-  - eapply match_program_no_more_functions in Heqo.
-    erewrite Heqo. auto.
-    eapply match_transform_program.
-Qed.
-
-
-Lemma Asmlabel_fn_stack_requirements_match: forall p tp,
-    Asmlabelgen.transf_program instr_size p = OK tp ->
-    fn_stack_requirements p = fn_stack_requirements tp.
-Proof.
-  intros. unfold fn_stack_requirements.  
-  eapply Axioms.extensionality. intros.
-  destr.
-  - eapply Globalenvs.Genv.find_funct_ptr_transf_partial in Heqo.
-    destruct Heqo as (tf & A & B).
-    erewrite A.
-    2:{
-      instantiate (1:= Asmlabelgen.transf_fundef instr_size).
-      eapply match_transform_partial_program.
-      unfold Asmlabelgen.transf_program in H. auto.
-    }
-    unfold Asmlabelgen.transf_fundef,transf_partial_fundef,Asmlabelgen.trans_function,transf_fundef in B.
-    destruct f. monadInv B. monadInv EQ. auto. inv B. auto.
-  - eapply match_program_no_more_functions in Heqo.
-    erewrite Heqo. auto.
-    eapply match_transform_partial_program.
-    unfold Asmlabelgen.transf_program in H. eauto.
-Qed.    
-
-
-Lemma AsmLiteral_fn_stack_requirements_match: forall p,
-    fn_stack_requirements p = fn_stack_requirements (AsmLiteral.transf_program p).
-Proof.
-  intros. unfold fn_stack_requirements.  
-  eapply Axioms.extensionality. intros.
-  destr.
-Admitted.
-
-Lemma Jumptable_fn_stack_requirements_match: forall p,
-    fn_stack_requirements p = fn_stack_requirements (Jumptablegen.transf_program instr_size p).
-Admitted.
-
 (* This should be an Axiom *)
-Lemma targetprinter_fn_stack_requirements_match: forall p tp,
+Axiom targetprinter_fn_stack_requirements_match: forall p tp,
     match_prog_targetprinter p tp ->
     fn_stack_requirements p = fn_stack_requirements tp.
-Proof.
-  intros.
-  unfold match_prog_targetprinter in H. unfold targetprinter in H.
-  unfold time in H.
-  simpl in H. 
-  destruct  AsmBuiltinInline.transf_program eqn: T1; simpl in H; try discriminate.
-  destruct  Asmlabelgen.transf_program eqn: T2; simpl in H; try discriminate.
-  inv H.
-
-  rewrite Pseudo_fn_stack_requirements_match.
-  rewrite Fixup_fn_stack_requirements_match.
-  erewrite (BuiltInline_fn_stack_requirements_match _ _ T1).
-  rewrite AsmLiteral_fn_stack_requirements_match.
-  rewrite AsmPseudo_fn_stack_requirements_match.
-  erewrite (Asmlabel_fn_stack_requirements_match _ _ T2).
-  erewrite Jumptable_fn_stack_requirements_match.
-  auto.
-Qed.
 
